src/Constructor.v
@@ -1,6 +1,11 @@
 (** * A constructor for simple types *)
 
+Require Import Coq.Program.Basics.
+Require Import Coq.Setoids.Setoid.
+Require Import Coq.Classes.RelationClasses.
+Require Import Coq.Classes.Morphisms.
 Require Export Codes.
+Require Import Diverge.
 Open Scope code_scope.
 
 Section exp.
@@ -32,13 +37,37 @@ Proof.
   hnf; unfold pair; beta_reduce; auto.
 Qed.
 
+Lemma pair_extensionality (Var : Set) (x y x' y' : Code Var) :
+  <<x, y>> [= <<x', y'>> <-> x [= x' /\ y [= y'.
+Proof.
+  unfold pair; beta_simpl; split.
+    intro H; split.
+      apply (code_le_ap_left _ _ _ K) in H; beta_simpl in H; auto.
+    apply (code_le_ap_left _ _ _ (K*I)) in H; beta_simpl in H; auto.
+  intros [Hx Hy]; auto.
+Qed.
+
 Definition sub_pair {Var : Set} (x : Code Var) := x [= <<TOP, TOP>>.
+
+Instance sub_pair_eq (Var : Set) :
+  Proper (code_eq ==> iff) (@sub_pair Var).
+Proof.
+  unfold sub_pair; intros x x' xx'; split; rewrite xx'; auto.
+Qed.
+
+Instance sub_pair_le (Var : Set) :
+  Proper (code_le --> impl) (@sub_pair Var).
+Proof.
+  unfold sub_pair; intros x x' xx' H. rewrite <- xx'; auto.
+Qed.
+
 Lemma sub_pair_pair (Var : Set) (x y : Code Var) : sub_pair <<x, y>>.
 Proof.
   unfold sub_pair, pair; eta_expand as f; beta_reduce.
   monotonicity; auto.
 Qed.
 
+(* FIXME is this true? *)
 Definition sub_pair_elim_intro {Var : Set} (x : Code Var) :
   sub_pair x -> x [= <<x*K, x*(K*I)>>.
 Proof.
@@ -46,6 +75,36 @@ Proof.
   intros H. (* eta_expand in H. FIXME eta_expand is borken *)
   eta_expand as f; beta_reduce.
 Admitted.
+
+Definition A_prop {Var : Set} (a : Code Var) :=
+  sub_pair a /\ forall s r, <<s, r>> [= a -> r o s [= I.
+
+Instance A_prop_le (Var : Set) : Proper (code_le --> impl) (@A_prop Var).
+Proof.
+  unfold A_prop; intros x x' xx'; intros [Hs Hl]; split.
+     rewrite <- xx'; auto.
+  intros s r H; rewrite <- xx' in *; auto.
+Qed.
+
+Instance A_prop_eq (Var : Set) : Proper (code_eq ==> iff) (@A_prop Var).
+Proof.
+  split; destruct H as [Hl Hr]; apply A_prop_le; auto.
+Qed.
+
+Ltac A_prop_pair :=
+  unfold A_prop; unfold sub_pair; split ;
+  [ try apply pair_extensionality; auto
+  | intros s r H;
+    apply pair_extensionality in H;
+    destruct H as [Hs Hr];
+    rewrite Hs; rewrite Hr
+  ].
+
+Lemma A_I_I (Var : Set) : A_prop (<<I, I>> : Code Var).
+Proof.
+  A_prop_pair; beta_eta.
+Qed.
+Hint Resolve A_I_I.
 
 Section raise.
   Context {Var : Set}.
@@ -57,7 +116,25 @@ Section raise.
 
   Definition pull := Eval compute in close (\x, \y, x || div * y).
   Definition push := Eval compute in close (\x, x * BOT).
+
+  Lemma lower_raise : lower o raise == I.
+  Proof. unfold lower, raise; beta_eta. Qed.
+
+  Lemma push_pull : push o pull == I.
+  Proof.
+    unfold push, pull; eta_expand; beta_simpl.
+    symmetry; apply code_le_eq_j.
+    fold (@div Var); code_simpl; auto.
+  Qed.
+
+  Lemma A_raise_lower : A_prop <<raise, lower>>.
+  Proof. A_prop_pair; apply lower_raise. Qed.
+
+  Lemma A_pull_push : A_prop <<pull, push>>.
+  Proof. A_prop_pair; apply push_pull. Qed.
 End raise.
+Hint Resolve A_raise_lower.
+Hint Resolve A_pull_push.
 
 Section compose.
   Context {Var : Set}.
@@ -74,8 +151,23 @@ Section compose.
     (\s, s*\a,\a', s*\b,\b', <<a' --> b, a --> b'>>).
 End compose.
 
+Lemma A_compose (Var : Set) (a : Code Var) : A_prop a -> A_prop (compose * a).
+Proof.
+  unfold A_prop, sub_pair; intros [Hs Ha].
+  unfold A_prop; unfold sub_pair; split.
+Admitted.
+Hint Resolve A_compose.
+
+Lemma A_conjugate (Var : Set) (a : Code Var) :
+  A_prop a -> A_prop (conjugate * a).
+Proof.
+  unfold A_prop, sub_pair; intros [Hs Ha].
+  unfold A_prop; unfold sub_pair; split.
+Admitted.
+Hint Resolve A_conjugate.
+
 Definition A {Var : Set} : Code Var :=
-  Eval compute in
+  (* Eval compute in *)
   Y * ( K * <<I, I>>
      || K * <<raise, lower>>
      || K * <<pull, push>>
@@ -91,22 +183,40 @@ Section A_example.
   Let A_example : Code Var := close (\\a,a'; a --> a').
 End A_example.
 
-Lemma A_sound (Var : Set) (r s : Code Var) : <<s, r>> [= A -> r o s [= I.
+Inductive A_above {Var : Set} : Code Var -> Prop :=
+  | A_above_below x y : x [= y -> A_above y -> A_above x
+  | A_above_i_i : A_above <<I, I>>
+  | A_above_raise_lower : A_above <<raise, lower>>
+  | A_above_pull_push : A_above <<pull, push>>
+  | A_above_compose a : A_above a -> A_above (compose * a)
+  | A_above_conjugate a : A_above a -> A_above (conjugate * a).
+
+Instance A_above_le (Var : Set) : Proper (code_le --> impl) (@A_above Var).
 Proof.
-  unfold A.
-  (*
-  apply Join_lub.
-  *)
-  (* unfold A_prop; split. *)
-  (*
-  unfold A_def.
-  apply Y_lfp.
-  intros y Hless.
-  repeat (rewrite J_beta || rewrite K_beta).
-  repeat apply J_lub.
-  *)
-  (* TODO *)
+  intros x x' xx' H; apply A_above_below with x; auto.
+Qed.
+
+Instance A_above_eq (Var : Set) : Proper (code_eq ==> iff) (@A_above Var).
+Proof.
+  split; destruct H as [Hl Hr]; apply A_above_le; auto.
+Qed.
+
+Lemma Y_lfp (Var : Set) (f b : Code Var) :
+  (forall x, x [= b -> f * x [= b) -> Y * f [= b.
+Proof.
 Admitted.
+
+Lemma A_above_A (Var : Set) (a : Code Var) : a [= A <-> A_above a.
+Proof.
+  (* TODO this needs some sort of least-fixed-point lemma *)
+Admitted.
+
+Lemma A_sound (Var : Set) (r s : Code Var) : <<s, r>> [= A -> A_prop <<s, r>>.
+Proof.
+  intros H; apply A_above_A in H.
+  induction H; auto.
+  rewrite H; auto.
+Qed.
 
 (** ** A strong characterization of [A] *)
 
@@ -115,32 +225,12 @@ Proof.
   (* TODO *)
 Admitted.
 
-Lemma A_I_I (Var : Set) : <<I, I>> [= (A : Code Var).
-Proof.
-  unfold A.
-  assert (I o I [= (I : Code Var)) as Heq.
-    eta_expand as x; beta_simpl; reflexivity.
-  (* TODO adapt the beta_eta tactic from Points to Codes:
-  TODO
-  apply Join_ub_eq with (i := restrict2_intro _ I I Heq).
-  *)
-Admitted.
-
 (*
 Lemma A_raise_lower : A_prop <<raise, lower>>.
 Proof.
   unfold A_prop; split;
   [ apply pair_is_pair
   | compute; eta_expand; beta_reduce; auto].
-Qed.
-
-Lemma A_pull_push : A_prop <<pull, push>>.
-Proof.
-  unfold A_prop; split.
-  apply pair_is_pair.
-  unfold pull.
-  freeze div in (compute; eta_expand; beta_reduce).
-  rewrite div_BOT; auto.
 Qed.
 
 Lemma A_compose : forall a, A_prop a -> A_prop (compose * a).
