src/Diverge.v
@@ -1,0 +1,62 @@
+(** * Proofs of divergence / nontermination *)
+
+Require Export Codes.
+Open Scope code_scope.
+
+Lemma beta_self_div (Var : Set) (x : Code Var) :
+  (forall ys z, beta (x ** ys) z -> x ** ys = z) -> ~ conv x.
+Proof.
+Admitted.
+
+Lemma beta_self_div' (Var : Set) (x : Code Var) :
+  conv x -> exists ys z, beta (x ** ys) z /\ x ** ys <> z.
+Proof.
+Admitted.
+
+Fixpoint probe {Var : Set} (n : nat) (x : Code Var) : Code Var :=
+  match n with
+  | 0%nat => x
+  | (Succ n')%nat => (probe n' x) * code_top
+  end.
+
+Lemma probe_bot_top (Var : Set) : forall n, probe n (@code_bot Var) <> TOP.
+Proof.
+  intros n; induction n; compute; fold (@probe Var); discriminate.
+Qed.
+
+Lemma approx_probe_bot_top (Var : Set) :
+  forall n, ~ approx (probe n (@code_bot Var)) TOP.
+Proof.
+  intros n H; induction n; auto.
+Admitted.
+
+Lemma div_probe_bot (Var : Set) :
+  forall n : nat, ~ conv (probe n (@code_bot Var)).
+Proof.
+  intros n H; inversion H.
+Admitted.
+
+Lemma div_bot (Var : Set) : div * BOT == (BOT : Code Var).
+Proof.
+  unfold div.
+  (* TODO this could be proved from an asymmetric definition of beta *)
+Admitted.
+Hint Rewrite div_bot : code_simpl.
+
+Section Omega.
+  Context {Var : Set}.
+  Let x := make_var Var 0.
+  Definition Omega := Eval compute in close ((\x, x * x) * (\x, x * x)).
+End Omega.
+
+Lemma code_le_omega_bot (Var : Set) : (@Omega Var) [= BOT.
+Proof.
+  unfold Omega, code_le, conv; intros Var' c f Ha.
+  induction Ha.
+  (* TODO this could be proved from an asymmetric definition of beta *)
+Admitted.
+
+Lemma code_eq_omega_bot (Var : Set) : (@Omega Var) == BOT.
+Proof.
+  split ; (apply code_le_omega_bot || auto).
+Qed.
